coq/Minimum.v
@@ -14,8 +14,66 @@ Open Scope nat_scope.
 
 Import ListNotations.
 
+(**************************************************)
+(* Key definitions *)
+
 Definition minimum (l : list tree) (t : tree) : Prop :=
   forall (t' : tree), flatten t' = l -> ht t <= ht t'.
+
+Theorem Lemma1 : forall (l s : list tree) (a b : tree) (sub : l = [a;b] ++ s),
+  lmp a b l -> exists (t : tree), siblings t a b -> minimum l t.
+Proof.
+Admitted.
+
+
+(**************************************************)
+(* Proving 'foldl1 join' gives minimum implicitly *)
+
+(* proving that the invariant holds when 'foldl1 join' is called,
+   assuming that 'fold_right step []' produces a strictly increasing list
+*)
+
+Theorem s_inc_two_lmp : forall (a b : tree) (l1 l2 : list tree), 
+  l1 = (a :: b :: l2) -> s_inc l1 -> lmp a b l1.
+Proof.
+  intros a b l1 l2 Cons Inc. rewrite Cons. 
+  destruct l2 as [|y]. apply lmp_pair. 
+    (* step *) apply lmp_threer. left. 
+    (* using the fact that the list is strictly increasing on both cases *)
+      split; rewrite Cons in Inc; inversion Inc; inversion H0.
+        assumption.
+        inversion H4. assumption. inversion H6. assumption.
+Qed.
+
+(* proving the the invariant that adding the join of a left-most pair in a strictly increasing list
+   preserves the fact that the left-most pair is still a local minimum pair.
+   assuming that foldl_left acts as it should 
+*)
+
+Theorem join_preserverse_leftmost_lmp : forall (t u v : tree) (ts : list tree),
+  s_inc (t :: u :: v :: ts) -> lmp (join t u) v (join t u :: v :: ts).
+Proof.
+ intros t u v ts Sinc. assert (H : ht (join t u) <= ht v). 
+   (* ass 1 *) simpl. replace (max (ht t) (ht u) + 1) with (S (max (ht t) (ht u))). apply lt_le_S. unfold max. remember (nat_compare (ht t) (ht u)) as R. destruct R.
+     inversion Sinc. inversion H0.  inversion H4. apply lt_trans with (m := ht u).  assumption. assumption.  apply lt_trans with (m := ht u). assumption. inversion H6. assumption. 
+     inversion Sinc. inversion H0. inversion H4.  assumption.  inversion H6. assumption. 
+     inversion Sinc. inversion H0.  inversion H4. apply lt_trans with (m := ht u).  assumption. assumption.  apply lt_trans with (m := ht u). assumption. inversion H6. assumption.
+   (* replace *) symmetry. apply NPeano.Nat.add_1_r.
+   induction ts. apply lmp_pair. 
+     (* step *) remember (nat_compare (ht (join t u)) (ht v)) as R1. destruct R1.
+       (* R1 = Eq *)apply lmp_threer. right. split. apply eq_ge. assumption. 
+                                       inversion Sinc. inversion H1. inversion H5. inversion H7. inversion H11. replace (ht (join t u)) with (ht v). assumption. symmetry. apply nat_compare_eq. symmetry. assumption. 
+                                                                                                                replace (ht (join t u)) with (ht v). inversion H13. assumption. symmetry. apply nat_compare_eq. symmetry. assumption.
+       (* R1 = LT *)apply lmp_threer. left. split. apply nat_compare_lt. symmetry. assumption. inversion Sinc. inversion H1.  inversion H5. inversion H7. inversion H11. assumption. inversion H13. assumption.
+       (* R1 = GT *)apply lmp_threer. contradict H. apply lt_not_le. apply nat_compare_gt. symmetry. assumption.
+Qed.
+
+(* Now given that Lemma1 proves that joining a lmp in a list of trees preserves the fact that we are on the way
+   of building a tree of minimum height, foldl1 creates a tree of minimum height *)
+
+
+(**************************************************)
+(* Proving 'foldl1 join' gives minimum explicitly *)
 
 Definition foldl1 (f : tree -> tree -> tree) (l : list tree) (P : l <> nil) : tree. 
   case l as [| x xs].
@@ -32,11 +90,6 @@ Admitted.
 
 Theorem join_preserves : forall (t1 t2 t3 : tree) (l s: list tree) (sub : l = [t1;t2] ++ s),
   lmp t1 t2 l -> minimum l t3 -> minimum (join t1 t2 :: s) t3.
-Proof.
-Admitted.
-
-Theorem Lemma1 : forall (l s : list tree) (a b : tree) (sub : l = [a;b] ++ s),
-  lmp a b l -> exists (t : tree), siblings t a b -> minimum l t.
 Proof.
 Admitted.
 
@@ -72,25 +125,3 @@ Admitted.
 Qed.
 *)
 
-(* proving the correctness of using join in fold1 *)
-(* assuming that foldl_left acts as it should this theorem proves that foldl1 preserves
-   the fact that the left-most pair of the list it works on is an lmp
- *)
-
-Theorem join_preserverse_leftmost_lmp : forall (t u v : tree) (ts : list tree),
-  s_inc (t :: u :: v :: ts) -> lmp (join t u) v (join t u :: v :: ts).
-Proof.
- intros t u v ts Sinc. assert (H : ht (join t u) <= ht v). 
-   (* ass 1 *) simpl. replace (max (ht t) (ht u) + 1) with (S (max (ht t) (ht u))). apply lt_le_S. unfold max. remember (nat_compare (ht t) (ht u)) as R. destruct R.
-     inversion Sinc. inversion H0.  inversion H4. apply lt_trans with (m := ht u).  assumption. assumption.  apply lt_trans with (m := ht u). assumption. inversion H6. assumption. 
-     inversion Sinc. inversion H0. inversion H4.  assumption.  inversion H6. assumption. 
-     inversion Sinc. inversion H0.  inversion H4. apply lt_trans with (m := ht u).  assumption. assumption.  apply lt_trans with (m := ht u). assumption. inversion H6. assumption.
-   (* replace *) symmetry. apply NPeano.Nat.add_1_r.
-   induction ts. apply lmp_pair. 
-     (* step *) remember (nat_compare (ht (join t u)) (ht v)) as R1. destruct R1.
-       (* R1 = Eq *)apply lmp_threer. right. split. apply eq_ge. assumption. 
-                                       inversion Sinc. inversion H1. inversion H5. inversion H7. inversion H11. replace (ht (join t u)) with (ht v). assumption. symmetry. apply nat_compare_eq. symmetry. assumption. 
-                                                                                                                replace (ht (join t u)) with (ht v). inversion H13. assumption. symmetry. apply nat_compare_eq. symmetry. assumption.
-       (* R1 = LT *)apply lmp_threer. left. split. apply nat_compare_lt. symmetry. assumption. inversion Sinc. inversion H1.  inversion H5. inversion H7. inversion H11. assumption. inversion H13. assumption.
-       (* R1 = GT *)apply lmp_threer. contradict H. apply lt_not_le. apply nat_compare_gt. symmetry. assumption.
-Qed.
