coq/SInc.v
@@ -41,10 +41,6 @@ Inductive s_inc : (list tree) -> Prop :=
 
 
 
-Theorem step_jointuv : forall (t u v : tree) (ts : list tree) (H3 : nat),
-  ht t >= ht u -> ht t < ht v -> H3 = (length (v :: ts)) -> step (join t u) (v :: ts) H3 = join t u :: v :: ts.
-Proof.
-Admitted.
 
 Theorem s_trans : forall (n m : nat),
   S n = S m -> n = m.
@@ -55,6 +51,7 @@ Theorem step_bigger : forall (t u : tree) (ts : list tree),
   s_inc (u :: ts) -> ht t >= ht u -> s_inc (step t (u :: ts) (length (u :: ts))). 
 Proof.
  intros t u ts Sinc t_ge_u.
+Admitted.
 
 Theorem tuvts_step : forall (t u v : tree) (ts : list tree),
   ht t < ht u -> step t (u :: v :: ts) (length (u :: v :: ts)) = t :: u :: v :: ts.
@@ -66,15 +63,26 @@ Proof.
     contradict t_lt_u. apply not_eq_r. apply gt_ge. assumption.
 Qed.
 
-Theorem tuvts_inc : forall (t u v : tree) (ts : list tree),
-  s_inc (u :: v :: ts) -> ht t < ht u -> s_inc (t :: u :: v :: ts).
+Theorem step_jointuv : forall (t u v : tree) (ts : list tree) (H3 : nat),
+  ht t >= ht u -> ht t < ht v -> H3 = (length (v :: ts)) -> step (join t u) (v :: ts) H3 = join t u :: v :: ts.
 Proof.
-intros t u v ts Sinc ht1. apply s_inc_cons. split.
-  assumption.
-  apply s_inc_cons. split.
-    inversion Sinc. assumption. inversion H0. assumption.
-    inversion Sinc. apply s_inc_sin. inversion H0. assumption.
-Qed.
+  intros t u v ts H3 t_ge_u t_lt_v Len.
+    remember (length (u :: v :: ts)) as R1. destruct R1. inversion HeqR1. 
+      remember (nat_compare (ht t) (ht u)) as R2. destruct R2. 
+        remember (nat_compare (ht t) (ht v)) as R3. destruct R3.
+          contradict t_lt_v. apply not_eq_r. apply eq_ge. assumption.
+(* how to unfold properly? *)
+Admitted.
+
+Theorem step_tjoinuv : forall (t u v : tree) (ts : list tree) (H3 : nat),
+  ht t >= ht u -> ht t >= ht v -> ht t < ht (join u v) -> step t (step (join u v) ts (length (v :: ts))) (length (v :: ts)) = t :: (join u v) :: ts.
+Proof.
+Admitted.
+
+Theorem step_jointjoinuv : forall (t u v : tree) (ts : list tree) (H3 : nat),
+  ht t >= ht u -> ht t >= ht v -> ht t >= ht (join u v) -> step t (step (join u v) ts (length (v :: ts))) (length (v :: ts)) = join t (join u v) :: ts.
+Proof.
+Admitted.
 
 Theorem jtuvts_step : forall (t u v : tree) (ts : list tree),
   ht t >= ht u -> ht t < ht v -> step t (u :: v :: ts) (length (u :: v :: ts)) = join t u :: v :: ts.
@@ -93,11 +101,64 @@ Proof.
         apply step_jointuv. assumption. assumption. simpl in *. apply s_trans. assumption.
 Qed.
 
-Theorem jtjuvts_step : forall (t u v : tree) (ts : list tree),
-  ht t >= ht u -> ht t >= ht v -> step t (u :: v :: ts) (length (u :: v :: ts)) = join t (join u v) :: ts.
+Theorem tjuvts_step : forall (t u v : tree) (ts : list tree),
+  ht t >= ht u -> ht t >= ht v -> ht t < ht (join u v) -> step t (u :: v :: ts) (length (u :: v :: ts)) = t :: (join u v) :: ts.
 Proof.
-Admitted.
+  intros t u v ts t_ge_u t_ge_v t_lt_juv. 
+  remember (length (u :: v :: ts)) as H3. destruct H3. simpl in HeqH3. inversion HeqH3. simpl.
+    remember (nat_compare (ht t) (ht u)) as H. destruct H. simpl.
+      remember (nat_compare (ht t) (ht v)) as H2. destruct H2.
+        replace (H3) with (length (v :: ts)). apply step_tjoinuv. apply H3. assumption. assumption. assumption. simpl in *. apply s_trans in HeqH3. symmetry. assumption.
+        contradict t_ge_v. apply lt_not_le. apply nat_compare_lt. symmetry. assumption.
+        replace (H3) with (length (v :: ts)). apply step_tjoinuv. apply H3. assumption. assumption. assumption. simpl in *. apply s_trans in HeqH3. symmetry. assumption.
+        contradict t_ge_u. apply lt_not_le. apply nat_compare_lt. symmetry. assumption.
+        remember (nat_compare (ht t) (ht v)) as R3. destruct R3.
+          replace (H3) with (length (v :: ts)). apply step_tjoinuv. apply H3. assumption. assumption. assumption. simpl in *. apply s_trans in HeqH3. symmetry. assumption.
+          contradict t_ge_v. apply lt_not_le. apply nat_compare_lt. symmetry. assumption.
+          replace (H3) with (length (v :: ts)). apply step_tjoinuv. apply H3. assumption. assumption. assumption. simpl in *. apply s_trans in HeqH3. symmetry. assumption.
+Qed.
 
+Theorem jtjuvts_step : forall (t u v : tree) (ts : list tree),
+  ht t >= ht u -> ht t >= ht v -> ht t >= ht (join u v) -> step t (u :: v :: ts) (length (u :: v :: ts)) = join t (join u v) :: ts.
+Proof.
+  intros t u v ts t_ge_u t_ge_v t_ge_juv.
+  remember (length (u :: v :: ts)) as H3. destruct H3. simpl in HeqH3. inversion HeqH3. simpl.
+    remember (nat_compare (ht t) (ht u)) as H. destruct H. simpl.
+      remember (nat_compare (ht t) (ht v)) as H2. destruct H2.
+        replace (H3) with (length (v :: ts)). apply step_jointjoinuv. apply H3. assumption. assumption. assumption. simpl in *. apply s_trans in HeqH3. symmetry. assumption.
+        contradict t_ge_v. apply lt_not_le. apply nat_compare_lt. symmetry. assumption.
+        replace (H3) with (length (v :: ts)). apply step_jointjoinuv. apply H3. assumption. assumption. assumption. simpl in *. apply s_trans in HeqH3. symmetry. assumption.
+        contradict t_ge_u. apply lt_not_le. apply nat_compare_lt. symmetry. assumption.
+        remember (nat_compare (ht t) (ht v)) as R3. destruct R3.
+          replace (H3) with (length (v :: ts)). apply step_jointjoinuv. apply H3. assumption. assumption. assumption. simpl in *. apply s_trans in HeqH3. symmetry. assumption.
+          contradict t_ge_v. apply lt_not_le. apply nat_compare_lt. symmetry. assumption.
+          replace (H3) with (length (v :: ts)). apply step_jointjoinuv. apply H3. assumption. assumption. assumption. simpl in *. apply s_trans in HeqH3. symmetry. assumption.
+Qed.
+
+Theorem tuvts_inc_alt : forall (t u v : tree) (ts : list tree),
+  s_inc (u :: v :: ts) -> ht t < ht u -> s_inc (step t (u :: v :: ts) (length (u :: v :: ts))).
+Proof.
+intros t u v ts Sinc ht1.
+  remember (length (u :: v :: ts)) as R1. destruct R1. inversion HeqR1. simpl.
+    remember (nat_compare (ht t) (ht u)) as R2. destruct R2. simpl.
+      remember (nat_compare (ht t) (ht v)) as R3. destruct R3.
+        contradict ht1. apply not_eq_r. apply eq_ge. assumption.
+        contradict ht1. apply not_eq_r. apply eq_ge. assumption.
+        contradict ht1. apply not_eq_r. apply eq_ge. assumption.
+        apply s_inc_cons. split; assumption.
+        contradict ht1. apply not_eq_r. apply gt_ge. assumption.
+Qed.
+
+Theorem tuvts_inc : forall (t u v : tree) (ts : list tree),
+  s_inc (u :: v :: ts) -> ht t < ht u -> s_inc (t :: u :: v :: ts).
+Proof.
+intros t u v ts Sinc ht1. apply s_inc_cons. split.
+  assumption.
+  apply s_inc_cons. split.
+    inversion Sinc. assumption. inversion H0. assumption.
+    inversion Sinc. apply s_inc_sin. inversion H0. assumption.
+Qed.
+(*
 Theorem jtuvts_inc2 : forall (t u v : tree) (ts : list tree),
   s_inc (u :: v :: ts) -> ht t >= ht u -> ht t < ht v -> ht (join t u) >= ht v -> s_inc (join (join t u) v :: ts).
 Proof.
@@ -113,20 +174,31 @@ Proof.
     contradict jtu_lt_v. apply not_eq_r. apply eq_ge. assumption.
     contradict jtu_lt_v. apply not_eq_r. apply gt_ge. assumption.
 Qed.
-
-Theorem jtuvts_inc1 : forall (t u v : tree) (ts : list tree),
+*)
+Theorem jtuvts_inc : forall (t u v : tree) (ts : list tree),
   s_inc (u :: v :: ts) -> ht t >= ht u -> ht t < ht v -> s_inc (step (join t u) (v :: ts) (length (v :: ts))).
 Proof.
-  intros t u v ts Sinc t_ge_u t_lt_v. remember (nat_compare (ht (join t u)) (ht v)) as H. destruct H.
-    induction ts. simpl. remember (nat_compare (max (ht t) (ht u) + 1) (ht v)) as H. destruct H.
-      apply s_inc_sin. apply s_inc_two. apply nat_compare_lt. symmetry. assumption. apply s_inc_sin.
-      (* step *) rewrite jtjuvts_step.
-        apply s_inc_cons.
-      
+  intros t u v ts Sinc t_ge_u t_lt_v. 
+    induction ts. 
+    (* base *)
+      simpl. remember (nat_compare (max (ht t) (ht u) + 1) (ht v)) as R1. destruct R1.
+        apply s_inc_sin.
+        apply s_inc_two. simpl. apply nat_compare_lt. symmetry. assumption.
+        apply s_inc_sin.
+    (* step *)
+      remember (nat_compare (ht (join t u)) (ht v)) as R. destruct R.
+        Focus 2. apply tuvts_inc_alt. inversion Sinc. inversion H0. assumption. apply nat_compare_lt. symmetry. assumption.
+        apply step_bigger. inversion Sinc. inversion H0. assumption. apply eq_ge. assumption.
+        apply step_bigger. inversion Sinc. inversion H0. assumption. apply gt_ge. assumption.
+Qed.
+
+Theorem tjuvts_inc : forall (t u v : tree) (ts : list tree),
+  s_inc (u :: v :: ts) -> ht t >= ht u -> ht t >= ht v -> ht t < ht (join u v) ->  s_inc (t :: (join u v) :: ts).
+Proof.
 Admitted.
 
 Theorem jtjuvts_inc : forall (t u v : tree) (ts : list tree),
-  s_inc (u :: v :: ts) -> ht t >= ht u -> ht t >= ht v -> s_inc (join t (join u v) :: ts).
+  s_inc (u :: v :: ts) -> ht t >= ht u -> ht t >= ht v -> ht t >= ht (join u v) -> s_inc (join t (join u v) :: ts).
 Proof.
 Admitted.
 
@@ -137,8 +209,8 @@ Proof.
   (* step *) induction l. simpl. intros t sIncA. remember (nat_compare (ht t) (ht a)) as H. destruct H; [apply s_inc_sin | apply s_inc_two; apply nat_compare_lt; symmetry; assumption | apply s_inc_sin].
     (* step *) intros t sInc. remember (nat_compare (ht t) (ht a)) as H. destruct H.
         remember (nat_compare (ht t) (ht a0)) as H2. destruct H2.
-          rewrite jtjuvts_step. apply jtjuvts_inc. assumption. apply eq_ge. assumption. 
-                                                 apply eq_ge. assumption.
+          rewrite tjuvts_step. apply tjuvts_inc. assumption. apply eq_ge. assumption. 
+                                                 apply eq_ge. assumption. simpl. unfold max. case (nat_compare (ht a) (ht a0)). 
                                                  apply eq_ge. assumption.
                                                  apply eq_ge. assumption.
           rewrite jtuvts_step. apply jtuvts_inc. assumption. apply eq_ge. assumption.
